zoo_parabs/vertex: Verify new, more flexible specification.

lib/zoo_parabs/vertex.ml
@@ -3,31 +3,45 @@
 *)
 
 type t =
-  { task: unit Pool.task;
+  { mutable task: bool Pool.task;
     mutable preds: int [@atomic];
     succs: t Mpmc_stack_2.t;
   }
 
 let create task =
+  let task =
+    match task with
+    | Some task ->
+        task
+    | None ->
+        Obj.magic ()
+  in
   { task;
     preds= 1;
     succs= Mpmc_stack_2.create ();
   }
 
+let get_task t =
+  t.task
+let set_task t task =
+  t.task <- task
+
 let precede t1 t2 =
   let succs1 = t1.succs in
   if not @@ Mpmc_stack_2.is_closed succs1 then (
     Atomic.Loc.fetch_and_add [%atomic.loc t2.preds] 1 |> ignore ;
-    if Mpmc_stack_2.push succs1 t2 then (
-      Atomic.Loc.fetch_and_add [%atomic.loc t2.preds] (-1) |> ignore ;
-      ()
-    )
+    if Mpmc_stack_2.push succs1 t2 then
+      Atomic.Loc.fetch_and_add [%atomic.loc t2.preds] (-1) |> ignore
   )
 
 let rec release ctx t =
   if Atomic.Loc.fetch_and_add [%atomic.loc t.preds] (-1) == 1 then
-    Pool.silent_async ctx (fun ctx -> run ctx t)
+    run ctx t
 and run ctx t =
-  t.task ctx ;
-  let succs = Mpmc_stack_2.close t.succs in
-  Clst.iter (fun succ -> release ctx succ) succs
+  Pool.silent_async ctx @@ fun ctx ->
+    t.preds <- 1 ;
+    if t.task ctx then
+      release ctx t
+    else
+      let succs = Mpmc_stack_2.close t.succs in
+      Clst.iter (fun succ -> release ctx succ) succs
